restructure Impl.Exponentiation
- make `one` as field of  `concrete_ops`
- precompute a table using `sqr` and `mul`
- take a precomputed table as argument in fixed-window methods

code/bignum/Hacl.Impl.MultiExponentiation.fst
@@ -8,19 +8,11 @@ open Lib.IntTypes
 open Lib.Buffer
 
 module ST = FStar.HyperStack.ST
-module B = LowStar.Buffer
-
-module LSeq = Lib.Sequence
-module BSeq = Lib.ByteSequence
 module Loops = Lib.LoopCombinators
 
-module LE = Lib.Exponentiation
-module SE = Spec.Exponentiation
+module S = Lib.Exponentiation
 module BD = Hacl.Bignum.Definitions
-module BN = Hacl.Bignum
-module SN = Hacl.Spec.Bignum
-module BB = Hacl.Bignum.Base
-module SB = Hacl.Spec.Bignum.Base
+module PT = Hacl.Impl.PrecompTable
 
 friend Hacl.Impl.Exponentiation
 
@@ -31,7 +23,11 @@ let lexp_double_fw_f_st
   (a_t:inttype_a)
   (len:size_t{v len > 0})
   (ctx_len:size_t)
-  (k:concrete_ops a_t len ctx_len) =
+  (k:concrete_ops a_t len ctx_len)
+  (l:size_window_t a_t len)
+  (table_len:table_len_t len)
+  (table_inv1:table_inv_t a_t len table_len)
+  (table_inv2:table_inv_t a_t len table_len) =
     ctx:lbuffer (uint_t a_t SEC) ctx_len
   -> a1:lbuffer (uint_t a_t SEC) len
   -> bLen:size_t
@@ -39,8 +35,6 @@ let lexp_double_fw_f_st
   -> b1:lbuffer (uint_t a_t SEC) bLen
   -> a2:lbuffer (uint_t a_t SEC) len
   -> b2:lbuffer (uint_t a_t SEC) bLen
-  -> l:size_t{0 < v l /\ v l < bits a_t /\ v l < 32}
-  -> table_len:size_t{1 < v table_len /\ v table_len * v len <= max_size_t /\ v table_len == pow2 (v l)}
   -> table1:lbuffer (uint_t a_t SEC) (table_len *! len)
   -> table2:lbuffer (uint_t a_t SEC) (table_len *! len)
   -> i:size_t{v i < v bBits / v l}
@@ -51,24 +45,20 @@ let lexp_double_fw_f_st
     live h acc /\ live h ctx /\ live h table1 /\ live h table2 /\
 
     eq_or_disjoint a1 a2 /\ disjoint a1 acc /\ disjoint a1 ctx /\
-    disjoint a1 table1 /\ disjoint a1 table2 /\ disjoint b1 acc /\
-    disjoint a2 acc /\ disjoint a2 ctx /\ disjoint a2 table1 /\ disjoint a2 table2 /\
+    disjoint b1 acc /\ disjoint a2 acc /\ disjoint a2 ctx /\
     disjoint b2 acc /\ disjoint acc ctx /\ disjoint acc table1 /\ disjoint acc table2 /\
-    disjoint ctx table1 /\ disjoint ctx table2 /\ eq_or_disjoint table1 table2 /\
 
     BD.bn_v h b1 < pow2 (v bBits) /\
     BD.bn_v h b2 < pow2 (v bBits) /\
     k.to.linv_ctx (as_seq h ctx) /\
     k.to.linv (as_seq h a1) /\ k.to.linv (as_seq h a2) /\
     k.to.linv (as_seq h acc) /\
-    (forall (j:nat{j < v table_len}).
-      precomp_table_inv len ctx_len k (as_seq h a1) table_len (as_seq h table1) j) /\
-    (forall (j:nat{j < v table_len}).
-      precomp_table_inv len ctx_len k (as_seq h a2) table_len (as_seq h table2) j))
+    table_inv1 (as_seq h a1) (as_seq h table1) /\
+    table_inv2 (as_seq h a2) (as_seq h table2))
   (ensures  fun h0 _ h1 -> modifies (loc acc) h0 h1 /\
     k.to.linv (as_seq h1 acc) /\
     k.to.refl (as_seq h1 acc) ==
-    SE.exp_double_fw_f #k.to.t_spec k.to.concr_ops
+    S.exp_double_fw_f #k.to.a_spec k.to.comm_monoid
       (k.to.refl (as_seq h0 a1)) (v bBits) (BD.bn_v h0 b1)
       (k.to.refl (as_seq h0 a2)) (BD.bn_v h0 b2) (v l) (v i) (k.to.refl (as_seq h0 acc)))
 
@@ -79,12 +69,18 @@ val lexp_double_fw_f:
   -> len:size_t{v len > 0}
   -> ctx_len:size_t
   -> k:concrete_ops a_t len ctx_len
-  -> lprecomp_get:lprecomp_get_st a_t len ctx_len k ->
-  lexp_double_fw_f_st a_t len ctx_len k
+  -> l:size_window_t a_t len
+  -> table_len:table_len_t len
+  -> table_inv1:table_inv_t a_t len table_len
+  -> table_inv2:table_inv_t a_t len table_len
+  -> pow_a_to_small_b1:pow_a_to_small_b_st a_t len ctx_len k l table_len table_inv1
+  -> pow_a_to_small_b2:pow_a_to_small_b_st a_t len ctx_len k l table_len table_inv2 ->
+  lexp_double_fw_f_st a_t len ctx_len k l table_len table_inv1 table_inv2
 
-let lexp_double_fw_f #a_t len ctx_len k lprecomp_get ctx a1 bLen bBits b1 a2 b2 l table_len table1 table2 i acc =
-  lexp_fw_f #a_t len ctx_len k lprecomp_get ctx a1 bLen bBits b1 l table_len table1 i acc;
-  lmul_acc_pow_a_bits_l len ctx_len k lprecomp_get ctx a2 bLen bBits b2 l table_len table2 i acc
+let lexp_double_fw_f #a_t len ctx_len k l table_len table_inv1 table_inv2
+  pow_a_to_small_b1 pow_a_to_small_b2 ctx a1 bLen bBits b1 a2 b2 table1 table2 i acc =
+  lexp_fw_f len ctx_len k l table_len table_inv2 pow_a_to_small_b2 ctx a2 bLen bBits b2 table2 i acc;
+  lmul_acc_pow_a_bits_l len ctx_len k l table_len table_inv1 pow_a_to_small_b1 ctx a1 bLen bBits b1 table1 i acc
 
 
 inline_for_extraction noextract
@@ -92,7 +88,11 @@ let lexp_double_fw_acc0_st
   (a_t:inttype_a)
   (len:size_t{v len > 0})
   (ctx_len:size_t)
-  (k:concrete_ops a_t len ctx_len) =
+  (k:concrete_ops a_t len ctx_len)
+  (l:size_window_t a_t len)
+  (table_len:table_len_t len)
+  (table_inv1:table_inv_t a_t len table_len)
+  (table_inv2:table_inv_t a_t len table_len) =
     ctx:lbuffer (uint_t a_t SEC) ctx_len
   -> a1:lbuffer (uint_t a_t SEC) len
   -> bLen:size_t
@@ -100,8 +100,6 @@ let lexp_double_fw_acc0_st
   -> b1:lbuffer (uint_t a_t SEC) bLen
   -> a2:lbuffer (uint_t a_t SEC) len
   -> b2:lbuffer (uint_t a_t SEC) bLen
-  -> l:size_t{0 < v l /\ v l < bits a_t /\ v l < 32}
-  -> table_len:size_t{1 < v table_len /\ v table_len * v len <= max_size_t /\ v table_len == pow2 (v l)}
   -> table1:lbuffer (uint_t a_t SEC) (table_len *! len)
   -> table2:lbuffer (uint_t a_t SEC) (table_len *! len)
   -> acc:lbuffer (uint_t a_t SEC) len ->
@@ -111,23 +109,19 @@ let lexp_double_fw_acc0_st
     live h acc /\ live h ctx /\ live h table1 /\ live h table2 /\
 
     eq_or_disjoint a1 a2 /\ disjoint a1 acc /\ disjoint a1 ctx /\
-    disjoint a1 table1 /\ disjoint a1 table2 /\ disjoint b1 acc /\
-    disjoint a2 acc /\ disjoint a2 ctx /\ disjoint a2 table1 /\ disjoint a2 table2 /\
+    disjoint b1 acc /\ disjoint a2 acc /\ disjoint a2 ctx /\
     disjoint b2 acc /\ disjoint acc ctx /\ disjoint acc table1 /\ disjoint acc table2 /\
-    disjoint ctx table1 /\ disjoint ctx table2 /\ eq_or_disjoint table1 table2 /\
 
     BD.bn_v h b1 < pow2 (v bBits) /\
     BD.bn_v h b2 < pow2 (v bBits) /\
     k.to.linv_ctx (as_seq h ctx) /\
     k.to.linv (as_seq h a1) /\ k.to.linv (as_seq h a2) /\
-    (forall (j:nat{j < v table_len}).
-      precomp_table_inv len ctx_len k (as_seq h a1) table_len (as_seq h table1) j) /\
-    (forall (j:nat{j < v table_len}).
-      precomp_table_inv len ctx_len k (as_seq h a2) table_len (as_seq h table2) j))
+    table_inv1 (as_seq h a1) (as_seq h table1) /\
+    table_inv2 (as_seq h a2) (as_seq h table2))
   (ensures  fun h0 _ h1 -> modifies (loc acc) h0 h1 /\
     k.to.linv (as_seq h1 acc) /\
     k.to.refl (as_seq h1 acc) ==
-    SE.exp_double_fw_acc0 #k.to.t_spec k.to.concr_ops
+    S.exp_double_fw_acc0 #k.to.a_spec k.to.comm_monoid
       (k.to.refl (as_seq h0 a1)) (v bBits) (BD.bn_v h0 b1)
       (k.to.refl (as_seq h0 a2)) (BD.bn_v h0 b2) (v l))
 
@@ -138,14 +132,19 @@ val lexp_double_fw_acc0:
   -> len:size_t{v len > 0}
   -> ctx_len:size_t
   -> k:concrete_ops a_t len ctx_len
-  -> lprecomp_get:lprecomp_get_st a_t len ctx_len k ->
-  lexp_double_fw_acc0_st a_t len ctx_len k
+  -> l:size_window_t a_t len
+  -> table_len:table_len_t len
+  -> table_inv1:table_inv_t a_t len table_len
+  -> table_inv2:table_inv_t a_t len table_len
+  -> pow_a_to_small_b1:pow_a_to_small_b_st a_t len ctx_len k l table_len table_inv1
+  -> pow_a_to_small_b2:pow_a_to_small_b_st a_t len ctx_len k l table_len table_inv2 ->
+  lexp_double_fw_acc0_st a_t len ctx_len k l table_len table_inv1 table_inv2
 
-let lexp_double_fw_acc0 #a_t len ctx_len k lprecomp_get ctx a1 bLen bBits b1 a2 b2 l table_len table1 table2 acc =
+let lexp_double_fw_acc0 #a_t len ctx_len k l table_len table_inv1 table_inv2 pow_a_to_small_b1 pow_a_to_small_b2 ctx a1 bLen bBits b1 a2 b2 table1 table2 acc =
   push_frame ();
   let tmp = create len (uint #a_t #SEC 0) in
-  lexp_fw_acc0 #a_t len ctx_len k lprecomp_get ctx a1 bLen bBits b1 l table_len table1 acc;
-  lexp_fw_acc0 #a_t len ctx_len k lprecomp_get ctx a2 bLen bBits b2 l table_len table2 tmp;
+  lexp_fw_acc0 len ctx_len k l table_len table_inv1 pow_a_to_small_b1 ctx a1 bLen bBits b1 table1 acc;
+  lexp_fw_acc0 len ctx_len k l table_len table_inv2 pow_a_to_small_b2 ctx a2 bLen bBits b2 table2 tmp;
   k.lmul ctx acc tmp acc;
   pop_frame ()
 
@@ -155,7 +154,11 @@ let lexp_double_fw_loop_st
   (a_t:inttype_a)
   (len:size_t{v len > 0})
   (ctx_len:size_t)
-  (k:concrete_ops a_t len ctx_len) =
+  (k:concrete_ops a_t len ctx_len)
+  (l:size_window_t a_t len)
+  (table_len:table_len_t len)
+  (table_inv1:table_inv_t a_t len table_len)
+  (table_inv2:table_inv_t a_t len table_len) =
     ctx:lbuffer (uint_t a_t SEC) ctx_len
   -> a1:lbuffer (uint_t a_t SEC) len
   -> bLen:size_t
@@ -163,8 +166,6 @@ let lexp_double_fw_loop_st
   -> b1:lbuffer (uint_t a_t SEC) bLen
   -> a2:lbuffer (uint_t a_t SEC) len
   -> b2:lbuffer (uint_t a_t SEC) bLen
-  -> l:size_t{0 < v l /\ v l < bits a_t /\ v l < 32}
-  -> table_len:size_t{1 < v table_len /\ v table_len * v len <= max_size_t /\ v table_len == pow2 (v l)}
   -> table1:lbuffer (uint_t a_t SEC) (table_len *! len)
   -> table2:lbuffer (uint_t a_t SEC) (table_len *! len)
   -> acc:lbuffer (uint_t a_t SEC) len ->
@@ -174,23 +175,19 @@ let lexp_double_fw_loop_st
     live h acc /\ live h ctx /\ live h table1 /\ live h table2 /\
 
     eq_or_disjoint a1 a2 /\ disjoint a1 acc /\ disjoint a1 ctx /\
-    disjoint a1 table1 /\ disjoint a1 table2 /\ disjoint b1 acc /\
-    disjoint a2 acc /\ disjoint a2 ctx /\ disjoint a2 table1 /\ disjoint a2 table2 /\
+    disjoint b1 acc /\ disjoint a2 acc /\ disjoint a2 ctx /\
     disjoint b2 acc /\ disjoint acc ctx /\ disjoint acc table1 /\ disjoint acc table2 /\
-    disjoint ctx table1 /\ disjoint ctx table2 /\ eq_or_disjoint table1 table2 /\
 
     BD.bn_v h b1 < pow2 (v bBits) /\
     BD.bn_v h b2 < pow2 (v bBits) /\
     k.to.linv_ctx (as_seq h ctx) /\
     k.to.linv (as_seq h a1) /\ k.to.linv (as_seq h a2) /\
     k.to.linv (as_seq h acc) /\
-    (forall (j:nat{j < v table_len}).
-      precomp_table_inv len ctx_len k (as_seq h a1) table_len (as_seq h table1) j) /\
-    (forall (j:nat{j < v table_len}).
-      precomp_table_inv len ctx_len k (as_seq h a2) table_len (as_seq h table2) j))
+    table_inv1 (as_seq h a1) (as_seq h table1) /\
+    table_inv2 (as_seq h a2) (as_seq h table2))
   (ensures  fun h0 _ h1 -> modifies (loc acc) h0 h1 /\ k.to.linv (as_seq h1 acc) /\
     k.to.refl (as_seq h1 acc) ==
-    Loops.repeati (v bBits / v l) (SE.exp_double_fw_f k.to.concr_ops (k.to.refl (as_seq h0 a1))
+    Loops.repeati (v bBits / v l) (S.exp_double_fw_f k.to.comm_monoid (k.to.refl (as_seq h0 a1))
       (v bBits) (BD.bn_v h0 b1) (k.to.refl (as_seq h0 a2)) (BD.bn_v h0 b2) (v l)) (k.to.refl (as_seq h0 acc)))
 
 
@@ -200,16 +197,21 @@ val lexp_double_fw_loop:
   -> len:size_t{v len > 0}
   -> ctx_len:size_t
   -> k:concrete_ops a_t len ctx_len
-  -> lprecomp_get:lprecomp_get_st a_t len ctx_len k ->
-  lexp_double_fw_loop_st a_t len ctx_len k
+  -> l:size_window_t a_t len
+  -> table_len:table_len_t len
+  -> table_inv1:table_inv_t a_t len table_len
+  -> table_inv2:table_inv_t a_t len table_len
+  -> pow_a_to_small_b1:pow_a_to_small_b_st a_t len ctx_len k l table_len table_inv1
+  -> pow_a_to_small_b2:pow_a_to_small_b_st a_t len ctx_len k l table_len table_inv2 ->
+  lexp_double_fw_loop_st a_t len ctx_len k l table_len table_inv1 table_inv2
 
-let lexp_double_fw_loop #a_t len ctx_len k lprecomp_get ctx a1 bLen bBits b1 a2 b2 l table_len table1 table2 acc =
+let lexp_double_fw_loop #a_t len ctx_len k l table_len table_inv1 table_inv2 pow_a_to_small_b1 pow_a_to_small_b2 ctx a1 bLen bBits b1 a2 b2 table1 table2 acc =
   let h0 = ST.get () in
 
   [@ inline_let]
-  let refl1 i : GTot k.to.t_spec = k.to.refl (as_seq h0 acc) in
+  let refl1 i : GTot k.to.a_spec = k.to.refl (as_seq h0 acc) in
   [@inline_let]
-  let spec (h:mem) = SE.exp_double_fw_f k.to.concr_ops (k.to.refl (as_seq h0 a1))
+  let spec (h:mem) = S.exp_double_fw_f k.to.comm_monoid (k.to.refl (as_seq h0 a1))
     (v bBits) (BD.bn_v h0 b1) (k.to.refl (as_seq h0 a2)) (BD.bn_v h0 b2) (v l) in
 
   [@inline_let]
@@ -217,82 +219,26 @@ let lexp_double_fw_loop #a_t len ctx_len k lprecomp_get ctx a1 bLen bBits b1 a2 
     modifies (loc acc) h0 h /\
     k.to.linv (as_seq h acc) /\
     k.to.refl (as_seq h acc) == Loops.repeati i (spec h0) (refl1 0) /\
-    (forall (j:nat{j < v table_len}).
-      precomp_table_inv len ctx_len k (as_seq h a1) table_len (as_seq h table1) j) /\
-    (forall (j:nat{j < v table_len}).
-      precomp_table_inv len ctx_len k (as_seq h a2) table_len (as_seq h table2) j) in
-
+    table_inv1 (as_seq h a1) (as_seq h table1) /\
+    table_inv2 (as_seq h a2) (as_seq h table2) in
 
   Loops.eq_repeati0 (v bBits / v l) (spec h0) (refl1 0);
   Lib.Loops.for 0ul (bBits /. l) inv
   (fun i ->
     Loops.unfold_repeati (v bBits / v l) (spec h0) (refl1 0) (v i);
-    lexp_double_fw_f len ctx_len k lprecomp_get ctx a1 bLen bBits b1 a2 b2 l table_len table1 table2 i acc
+    lexp_double_fw_f len ctx_len k l table_len table_inv1 table_inv2 pow_a_to_small_b1 pow_a_to_small_b2 ctx a1 bLen bBits b1 a2 b2 table1 table2 i acc
   )
 
 
-inline_for_extraction noextract
-let lexp_double_fw_gen_st
-  (a_t:inttype_a)
-  (len:size_t{v len > 0})
-  (ctx_len:size_t)
-  (k:concrete_ops a_t len ctx_len) =
-    ctx:lbuffer (uint_t a_t SEC) ctx_len
-  -> a1:lbuffer (uint_t a_t SEC) len
-  -> bLen:size_t
-  -> bBits:size_t{(v bBits - 1) / bits a_t < v bLen}
-  -> b1:lbuffer (uint_t a_t SEC) bLen
-  -> a2:lbuffer (uint_t a_t SEC) len
-  -> b2:lbuffer (uint_t a_t SEC) bLen
-  -> l:size_t{0 < v l /\ v l < bits a_t /\ v l < 32}
-  -> table_len:size_t{1 < v table_len /\ v table_len * v len <= max_size_t /\ v table_len == pow2 (v l)}
-  -> table1:lbuffer (uint_t a_t SEC) (table_len *! len)
-  -> table2:lbuffer (uint_t a_t SEC) (table_len *! len)
-  -> acc:lbuffer (uint_t a_t SEC) len ->
-  Stack unit
-  (requires fun h ->
-    live h a1 /\ live h b1 /\ live h a2 /\ live h b2 /\
-    live h acc /\ live h ctx /\ live h table1 /\ live h table2 /\
-
-    eq_or_disjoint a1 a2 /\ disjoint a1 acc /\ disjoint a1 ctx /\
-    disjoint a1 table1 /\ disjoint a1 table2 /\ disjoint b1 acc /\
-    disjoint a2 acc /\ disjoint a2 ctx /\ disjoint a2 table1 /\ disjoint a2 table2 /\
-    disjoint b2 acc /\ disjoint acc ctx /\ disjoint acc table1 /\ disjoint acc table2 /\
-    disjoint ctx table1 /\ disjoint ctx table2 /\ eq_or_disjoint table1 table2 /\
-
-    BD.bn_v h b1 < pow2 (v bBits) /\
-    BD.bn_v h b2 < pow2 (v bBits) /\
-    k.to.linv_ctx (as_seq h ctx) /\
-    k.to.linv (as_seq h a1) /\ k.to.linv (as_seq h a2) /\
-    k.to.linv (as_seq h acc) /\ k.to.refl (as_seq h acc) == k.to.concr_ops.SE.one () /\
-    (forall (j:nat{j < v table_len}).
-      precomp_table_inv len ctx_len k (as_seq h a1) table_len (as_seq h table1) j) /\
-    (forall (j:nat{j < v table_len}).
-      precomp_table_inv len ctx_len k (as_seq h a2) table_len (as_seq h table2) j))
-  (ensures  fun h0 _ h1 -> modifies (loc acc) h0 h1 /\
-    k.to.linv (as_seq h1 acc) /\
-    k.to.refl (as_seq h1 acc) ==
-    SE.exp_double_fw k.to.concr_ops
-      (k.to.refl (as_seq h0 a1)) (v bBits) (BD.bn_v h0 b1)
-      (k.to.refl (as_seq h0 a2)) (BD.bn_v h0 b2) (v l))
-
-
-inline_for_extraction noextract
-val lexp_double_fw_gen_:
-    #a_t:inttype_a
-  -> len:size_t{v len > 0}
-  -> ctx_len:size_t
-  -> k:concrete_ops a_t len ctx_len
-  -> lprecomp_get:lprecomp_get_st a_t len ctx_len k ->
-  lexp_double_fw_gen_st a_t len ctx_len k
-
-let lexp_double_fw_gen_ #a_t len ctx_len k lprecomp_get ctx a1 bLen bBits b1 a2 b2 l table_len table1 table2 acc =
+let mk_lexp_double_fw_tables #a_t len ctx_len k l table_len table_inv1 table_inv2 pow_a_to_small_b1 pow_a_to_small_b2 ctx a1 bLen bBits b1 a2 b2 table1 table2 res =
   assert (v (bBits %. l) == v bBits % v l);
   if bBits %. l <> 0ul then
-    lexp_double_fw_acc0 len ctx_len k lprecomp_get ctx a1 bLen bBits b1 a2 b2 l table_len table1 table2 acc;
+    lexp_double_fw_acc0 len ctx_len k l table_len table_inv1 table_inv2 pow_a_to_small_b1 pow_a_to_small_b2 ctx a1 bLen bBits b1 a2 b2 table1 table2 res
+  else k.lone ctx res;
 
-  lexp_double_fw_loop #a_t len ctx_len k lprecomp_get ctx a1 bLen bBits b1 a2 b2 l table_len table1 table2 acc
+  lexp_double_fw_loop #a_t len ctx_len k l table_len table_inv1 table_inv2 pow_a_to_small_b1 pow_a_to_small_b2 ctx a1 bLen bBits b1 a2 b2 table1 table2 res
 
+//-----------------------------------
 
 inline_for_extraction noextract
 val lexp_double_fw_gen:
@@ -300,48 +246,55 @@ val lexp_double_fw_gen:
   -> len:size_t{v len > 0}
   -> ctx_len:size_t
   -> k:concrete_ops a_t len ctx_len
-  -> lprecomp_get:lprecomp_get_st a_t len ctx_len k ->
-  lexp_double_fw_st a_t len ctx_len k
+  -> l:size_window_t a_t len
+  -> table_len:table_len_t len{1 < v table_len /\ v table_len == pow2 (v l)}
+  -> lprecomp_get:pow_a_to_small_b_st a_t len ctx_len k l table_len
+                   (table_inv_precomp len ctx_len k l table_len) ->
+  lexp_double_fw_st a_t len ctx_len k l
 
 #push-options "--z3rlimit 150"
-let lexp_double_fw_gen #a_t len ctx_len k lprecomp_get ctx a1 bLen bBits b1 a2 b2 acc l =
+let lexp_double_fw_gen #a_t len ctx_len k l table_len lprecomp_get ctx a1 bLen bBits b1 a2 b2 acc =
   push_frame ();
-  Math.Lemmas.pow2_lt_compat 32 (v l);
+  lemma_pow2_is_divisible_by_2 (v l);
+  let table1 = create (table_len *! len) (uint #a_t #SEC 0) in
+  PT.lprecomp_table #a_t len ctx_len k ctx a1 table_len table1;
+  let h0 = ST.get () in
+  assert (table_inv_precomp len ctx_len k l table_len (as_seq h0 a1) (as_seq h0 table1));
+
+  let table2 = create (table_len *! len) (uint #a_t #SEC 0) in
+  PT.lprecomp_table #a_t len ctx_len k ctx a2 table_len table2;
+  let h1 = ST.get () in
+  assert (table_inv_precomp len ctx_len k l table_len (as_seq h1 a1) (as_seq h1 table1));
+  assert (table_inv_precomp len ctx_len k l table_len (as_seq h1 a2) (as_seq h1 table2));
+
+  mk_lexp_double_fw_tables len ctx_len k l table_len
+    (table_inv_precomp len ctx_len k l table_len)
+    (table_inv_precomp len ctx_len k l table_len)
+    lprecomp_get lprecomp_get ctx a1 bLen bBits b1 a2 b2 table1 table2 acc;
+  pop_frame ()
+#pop-options
+
+
+let lexp_double_fw_vartime #a_t len ctx_len k l ctx a1 bLen bBits b1 a2 b2 acc =
   [@inline_let]
   let table_len = 1ul <<. l in
   assert (v table_len == pow2 (v l));
   Math.Lemmas.pow2_le_compat (v l) 1;
   assert (1 < v table_len /\ v table_len * v len <= max_size_t);
 
-  let table1 = create (table_len *! len) (uint #a_t #SEC 0) in
-  update_sub table1 0ul len acc;
-  lprecomp_table #a_t len ctx_len k ctx a1 table_len table1;
-  let h = ST.get () in
-  assert (forall (j:nat{j < v table_len}).
-      precomp_table_inv len ctx_len k (as_seq h a1) table_len (as_seq h table1) j);
-
-  let table2 = create (table_len *! len) (uint #a_t #SEC 0) in
-  update_sub table2 0ul len acc;
-  lprecomp_table #a_t len ctx_len k ctx a2 table_len table2;
-  let h = ST.get () in
-  assert (forall (j:nat{j < v table_len}).
-      precomp_table_inv len ctx_len k (as_seq h a1) table_len (as_seq h table1) j);
-  assert (forall (j:nat{j < v table_len}).
-      precomp_table_inv len ctx_len k (as_seq h a2) table_len (as_seq h table2) j);
-
-  lexp_double_fw_gen_ #a_t len ctx_len k lprecomp_get
-    ctx a1 bLen bBits b1 a2 b2 l table_len table1 table2 acc;
-  pop_frame ()
-#pop-options
+  lexp_double_fw_gen len ctx_len k l table_len
+    (lprecomp_get_vartime len ctx_len k l table_len)
+    ctx a1 bLen bBits b1 a2 b2 acc
 
 
-let lexp_double_fw_vartime #a_t len ctx_len k ctx a1 bLen bBits b1 a2 b2 acc w =
-  lexp_double_fw_gen #a_t len ctx_len k
-    (lprecomp_get_vartime #a_t len ctx_len k)
-    ctx a1 bLen bBits b1 a2 b2 acc w
+let lexp_double_fw_consttime #a_t len ctx_len k l ctx a1 bLen bBits b1 a2 b2 acc =
+  [@inline_let]
+  let table_len = 1ul <<. l in
+  assert (v table_len == pow2 (v l));
+  Math.Lemmas.pow2_le_compat (v l) 1;
+  assert (1 < v table_len /\ v table_len * v len <= max_size_t);
 
+  lexp_double_fw_gen len ctx_len k l table_len
+    (lprecomp_get_consttime len ctx_len k l table_len)
+    ctx a1 bLen bBits b1 a2 b2 acc
 
-let lexp_double_fw_consttime #a_t len ctx_len k ctx a1 bLen bBits b1 a2 b2 acc w =
-  lexp_double_fw_gen #a_t len ctx_len k
-    (lprecomp_get_consttime #a_t len ctx_len k)
-    ctx a1 bLen bBits b1 a2 b2 acc w
